new definition of Informative, everything compiles

extraction/theories/Extract.v
@@ -50,29 +50,35 @@ Axiom is_type_or_proof_spec : forall (Sigma : global_context) (Gamma : context) 
 (*        ret (Universe.is_prop s). *)
 (* End IsType. *)
 
-Fixpoint all_args t :=
-  match t with
-  | tProd _ t1 t2 => t1 :: all_args t2
-  | _ => []
-  end.  
+(* Fixpoint all_args t := *)
+(*   match t with *)
+(*   | tProd _ t1 t2 => t1 :: all_args t2 *)
+(*   | _ => [] *)
+(*   end.   *)
 
-Fixpoint target_type t :=
-  match t with
-  | tProd _ t1 t2 => target_type t2
-  | _ => t
-  end.
+(* Fixpoint target_type t := *)
+(*   match t with *)
+(*   | tProd _ t1 t2 => target_type t2 *)
+(*   | _ => t *)
+(*   end. *)
 
-Definition Is_Singleton (Σ : global_context) mdecl ind idecl univ :=
-    #|ind_ctors idecl| <= 1 /\
-    forall cdecl i,
-      declared_constructor (fst Σ) mdecl idecl (ind, i) cdecl ->
-      Forall (fun t => match t with tSort u => is_prop_sort u | _ => False end) (skipn (ind_npars mdecl) (all_args (type_of_constructor mdecl cdecl (ind, i) univ))).
+Definition Is_proof Σ Γ t := ∑ T u, Σ ;;; Γ |- t : T × Σ ;;; Γ |- T : tSort u × is_prop_sort u.
 
-Definition Informative (Σ : global_context) (ind : inductive) (univ : universe_instance) :=
-  forall mdecl idecl u,
+Lemma Is_Type_or_Proof_Proof Σ Γ t :
+  Is_proof Σ Γ t -> Is_Type_or_Proof Σ Γ t.
+Proof.
+  intros. destruct X as (? & ? & ? & ? & ?). exists x. split. eauto. right. eauto.
+Qed.
+
+Definition Informative (Σ : global_context) (ind : inductive) :=
+  forall mdecl idecl,
     declared_inductive (fst Σ) mdecl ind idecl ->
-    target_type (ind_type idecl) = tSort u ->
-    is_prop_sort u -> Is_Singleton Σ mdecl ind idecl univ.
+    forall Γ args u n Σ',
+      wf Σ' ->
+      PCUICWeakeningEnv.extends Σ Σ' ->
+      Is_proof Σ' Γ (mkApps (tConstruct ind n u) args) ->  
+       #|ind_ctors idecl| <= 1 /\
+       squash (All (Is_proof Σ' Γ) (skipn (ind_npars mdecl) args)).
 
 Module E := EAst.
 Local Notation Ret t := t.
@@ -238,9 +244,8 @@ Inductive erases (Σ : global_context) (Γ : context) : term -> E.term -> Prop :
     erases Σ Γ (tConst kn u) (E.tConst kn)
 | erases_tConstruct kn k n :
     erases Σ Γ (tConstruct kn k n) (E.tConstruct kn k)
-| erases_tCase1 ind npar T c brs c' brs' u args :
-    Σ ;;; Γ |- c : mkApps (tInd ind u) args -> (* This is to make sure we have the right u. *)
-    Informative Σ ind u ->
+| erases_tCase1 ind npar T c brs c' brs' :
+    Informative Σ ind ->
     erases Σ Γ c c' ->
     All2 (fun x x' => erases Σ Γ (snd x) (snd x') × fst x = fst x') brs brs' ->
     erases Σ Γ (tCase (ind, npar) T c brs) (E.tCase (ind, npar) c' brs')
@@ -251,10 +256,9 @@ Inductive erases (Σ : global_context) (Γ : context) : term -> E.term -> Prop :
 (*     erases Σ Γ c E.tBox -> *)
 (*     erases Σ Γ x x' -> *)
 (*     erases Σ Γ (tCase ip T c ((n, x) :: brs)) (mkAppBox x' n) *)
-| erases_tProj p c c' u args :
+| erases_tProj p c c' :
     let ind := fst (fst p) in
-    Σ ;;; Γ |- c : mkApps (tInd ind u) args ->
-    Informative Σ ind u ->
+    Informative Σ ind ->
     erases Σ Γ c c' ->
     erases Σ Γ (tProj p c) (E.tProj p c')
 | erases_tFix mfix n mfix' :
